An ODE of the form $du(t)/dt = a \cdot c(t) \cdot u(t) + b$, where the state variable $u(t)$ changes over time.
For a system governed by the control variable $c(t)$, the state variable $u(t)$ follows the differential equation,  $du/dt = a \cdot c(t) \cdot u + b$.
The ordinary differential equation is expressed as $du(t)/dt = a \cdot c(t) \cdot u(t) + b$ with $u(t)$ the state variable and $c(t)$ the control variable.
State variable $u(t)$ and control variable $c(t)$ are linked by the ODE $du(t)/dt = a \cdot c(t) \cdot u(t) + b$.
The rate at which $u(t)$ changes, as described by this ODE, is determined by the variables $a$, $c(t)$, $u(t)$, and $b$.
The function $u(t)$ evolves over time accord to the differential equation $du(t)/dt = a \cdot c(t) \cdot u(t) + b$.
The ODE $du(t)/dt = a \cdot c(t) \cdot u(t) + b$ gives the rate of change of state variable $u (t)$.
Our ODE can be written as $\frac{du(t)}{dt} = a \cdot c(t) \cdot u(t) + b$.
The way in which $u(t)$ depends on time is described using $\frac{du(t)}{dt} = a \cdot c(t) \cdot u(t) + b$.
The time derivative of state variable, $u(t)$, follows the ordinary differential equation: $du(t)/dt = a \cdot c(t) \cdot u(t) + b$.
Consider an ordinary differential equation given as $\frac{du(t)}{dt} = a \cdot c(t) \cdot u(t) + b$.
 The ODE represents the time evolution of the state variable $u(t)$ influenced by the control variable $c(t)$.
The change rate of $u(t)$ relative to time is represented by $a \cdot c(t) \cdot u(t) + b$.
The differential equation $du(t)/dt = a \cdot c(t) \cdot u(t) + b$ describes the relationship between the time variation of $u(t)$ and the control variable $c(t)$.
This ODE is defined by the state variable $u$ and the control variable $c$ in the form of $\frac{du(t)}{dt} = a \cdot c(t) \cdot u(t) + b$.
The instantaneous rate of change of $u(t)$ is given by $du(t)/dt = a \cdot c(t) \cdot u(t) + b$.
This is an ordinary differential equation in the form of $du(t)/dt = a \cdot c(t) \cdot u(t) + b$.
Under the ordinary differential equation $\frac{du}{dt} = a \cdot c(t) \cdot u + b$, $u(t)$ is the state variable and $c(t)$ is the control variable.
The ODE describes how the state variable $u(t)$ changes over time as a function of itself and the control variable $c(t)$ via the relation $du(t)/dt = a \cdot c(t) \cdot u(t) + b$.
The ODE is given by the time derivative of $u$ which is equal to $b$ plus the product of $a, c(t)$ and $u(t)$.
We describe the ODE as $\frac{du(t)}{dt} = a \cdot c(t) \cdot u(t) + b$, where $u(t)$ and $c(t)$ are the state and control variables.
The ODE involves a control function $c(t)$ influencing the rate of change of $u(t)$.
The ODE can be described as $du(t)/dt = a \cdot c(t) \cdot u(t) + b$.
The dynamics of state variable $u(t)$ over time are dictated by $\frac{du(t)}{dt} = a \cdot c(t) \cdot u(t) + b$.
The rate of change of the function $u(t)$ is expressed as $du(t)/dt = a \cdot c(t) \cdot u(t) + b$ in this ODE.
State variable $u$ fluctuates based on the changes of the control variable $c$ in this ODE.
The ODE representing $u(t)$'s change rate is $du(t)/dt = a \cdot c(t) \cdot u(t) + b$, where $c(t)$ is a control variable.
The change in the state variable $u$ with respect to time can be expressed through the ODE $du(t)/dt = a \cdot c(t) \cdot u(t) + b$.
For a system described by a state variable $u(t)$ and a control variable $c(t)$, the ODE takes the form $\frac{du(t)}{dt} = a \cdot c(t) \cdot u(t) + b$.
The ODE $\frac{du(t)}{dt} = a \cdot c(t) \cdot u(t) + b$ relates $u(t)$'s rate of change to $c(t)$.
The temporal evolution of the variable $u(t)$ is dictated by an ODE, specifically $du(t)/dt = a \cdot c(t) \cdot u(t) + b$.
In this differential equation, the rate of change of $u$ is governed by the product $c(t) \cdot u(t)$ scaled by $a$, with an offset of $b$.
This differential equation is described by $\frac{du(t)}{dt} = a \cdot c(t) \cdot u(t) + b$ where $u(t)$ is the state variable and $c(t)$ is the control variable.
The rate of change of $u(t)$ is governed by an ordinary differential equation $du(t)/dt = a \cdot c(t) \cdot u(t) + b$.
The time-varying variables $u(t)$ and $c(t)$ are related by the ordinary differential equation $du(t)/dt = a \cdot c(t) \cdot u(t) + b$.
In this ODE, the growth rate of the population $u(t)$ is expressed as $du(t)/dt = a \cdot c(t) \cdot u(t) + b$.
The other form of the ODE can be expressed as ${du}/{dt} = a \cdot c \cdot u + b$ for the state variable $u(t)$.
The ODE exhibits that the derivative of the state variable $u$, relative to time $t$, is equivalent to the sum of the product $a \cdot c(t) \cdot u(t)$ and the constant $b$.
An ODE with a state variable $u(t)$ and a control variable $c(t)$. 
Our system is governed by the ordinary differential equation $du/dt = a \cdot c(t) \cdot u + b$; where $u(t)$ is our state variable and $c(t)$ is our control variable.
For state variable $u(t)$ and control variable $c(t)$, the ODE presents as $du(t)/dt = a \cdot c(t) \cdot u(t) + b$.
An ODE that describes observations on how $u(t)$ transforms is given by $du(t)/dt = a \cdot c(t) \cdot u(t) + b$.
The ordinary differential equation is represented as $du/dt = a \cdot c \cdot u + b$ where $u(t)$ is the state variable and $c(t)$ is the control variable.
Using an ODE, the state variable $u(t)$ can be expressed as $\frac{du(t)}{dt} = a \cdot c(t) \cdot u(t) + b$.
The ODE is modelled as $\frac{du(t)}{dt} = a \cdot c(t) \cdot u(t) + b$.
Consider the ordinary differential equation of the form $du(t)/dt=a \cdot c(t) \cdot u(t) + b$ where $u$ and $c$ are functions of time $t$.
The ODE contains a single time-dependent state variable $u(t)$.
An ordinary differential equation that describes the relationship of $u(t)$ and $c(t)$ is $du(t)/dt = a \cdot c(t) \cdot u(t) + b$.
We have an ordinary differential equation of the form $du(t)/dt = a \cdot c(t) \cdot u(t) + b$.
The rate at which state variable $u(t)$ changes, is prescribed by the differential relationship $du(t)/dt = a \cdot c(t) \cdot u(t) + b$.
For variable $u(t)$, the corresponding ODE is $du(t)/dt = a \cdot c(t) \cdot u(t) + b$.
$u(t)$'s rate of change is dependent on the state variable $u(t)$ and the control variable $c(t)$.
The ordinary differential equation $\frac{du(t)}{dt} = a \cdot c(t) \cdot u(t) + b$ describes the state variable $u(t)$ in time.
Function $u(t)$ varies over time based on the equation: $\frac{du(t)}{dt} = a \cdot c(t) \cdot u(t) + b$.
The given ODE is expressed as $du(t)/dt = a \cdot c(t) \cdot u(t) + b$ where $u(t)$ is a function of time.
The ODE is formulated in terms of the state variable $u$ and the control variable $c$, with the generic parameters $a$ and $b$.
The quantity $u(t)$ evolves according to the ordinary differential equation $\frac{du(t)}{dt} = a \cdot c(t) \cdot u(t) + b$.
We are looking at an ODE with $du(t)/dt = a \cdot c(t) \cdot u(t) + b$.
The ODE expresses the change of $u(t)$ at the rate of $a \cdot c(t) \cdot u(t) + b$.
In ODE form, state variable $u(t)$ can be presented as $\frac{du(t)}{dt} = a \cdot c(t) \cdot u(t) + b$.
The ODE that describes how state variable $u(t)$ evolves over time is $\frac{du(t)}{dt} = a \cdot c(t) \cdot u(t) + b$.
Given the control variable $c(t)$, the rate of $u(t)$ changes as $du(t)/dt = a \cdot c(t) \cdot u(t) + b$.
The manner in which $u(t)$ alters over time is given by the ODE $du(t)/dt = a \cdot c(t) \cdot u(t) + b$.
State variable $u(t)$'s temporal evolution is encapsulated by $\frac{du(t)}{dt} = a \cdot c(t) \cdot u(t) + b$.
Examining an ODE where the derivative of $u(t)$ is given by $du(t)/dt = a \cdot c(t) \cdot u(t) + b$.
The state variable $u(t)$ in our ODE is subject to a change rate of $a \cdot c(t) \cdot u(t) + b$.
The ordinary differential equation models the change in state $u$ over time via $du(t)/dt = a \cdot c(t) \cdot u(t) + b$.
The changes in function $u(t)$ are determined by the equation $du(t)/dt = a \cdot c(t) \cdot u(t) + b$.
Consider an ordinary differential equation given by $\frac{du(t)}{dt} = a \cdot c(t) \cdot u(t) + b$.
The mathematical model covers the changing rate of $u(t)$ with $c(t)$ as $a \cdot c(t) \cdot u(t) + b$.
If we introduce $u(t)$ as the state variable, and $c(t)$ as the control variable, we have the following ODE: $\frac{du(t)}{dt} = a \cdot c(t) \cdot u(t) + b$.
Here, the symbol $a \cdot c(t) \cdot u(t) + b$ represents the rate at which $u(t)$ is changing.
ODE is characterized by a state variable $u$ and control variable $c$.
Time-based state variable $u(t)$ is governed by $du(t)/dt = a \cdot c(t) \cdot u(t) + b$.
The ODE governing the behaviour of $u(t)$ with respect to time is $\frac{du(t)}{dt} = a \cdot c(t) \cdot u(t) + b$.
The function $u(t)$ undergoes changes as per the ODE: $du(t)/dt = a \cdot c(t) \cdot u(t) + b$.
In this ODE, $u$ changes at a rate given by $a \cdot c(t) \cdot u(t) + b$.
This ordinary differential equation has the form $\frac{du(t)}{dt} = a \cdot c(t) \cdot u(t) + b$.
The manner in which $u(t)$ varies with time can be formulated as $\frac{du(t)}{dt} = a \cdot c(t) \cdot u(t) + b$.
The ODE in question is of the form $\frac{du(t)}{dt} = a \cdot c(t) \cdot u(t) + b$ and exhibits the change of $u(t)$ over time with $c(t)$ as a potential influencer.
A state variable $u(t)$ evolves over time according to the differential equation $du(t)/dt = a \cdot c(t) \cdot u(t) + b$.
The ODE $\frac{du(t)}{dt} = a \cdot c(t) \cdot u(t) + b$ describes the change of state variable $u(t)$ in terms of control variable $c(t)$.
$u(t)$ is a state variable changing with the rate given by the ODE $du(t)/dt = a \cdot c(t) \cdot u(t) + b$ in control of variable $c(t)$.
The derivative of the function $u(t)$ is described by $du(t)/dt = a \cdot c(t) \cdot u(t) + b$.
We have an ODE of the form $\frac{du}{dt} = a \cdot c(t) \cdot u + b$ for the variable $u$ with control variable $c$.
The rate of change of the variable $u(t)$ is controlled by the equation $du(t)/dt = a \cdot c(t) \cdot u(t) + b$.
The ODE can be formulated as $du(t)/dt = a \cdot c(t) \cdot u(t) + b$.
An ODE is given by $\frac{du}{dt} = a \cdot c \cdot u + b$ where $u(t)$ is the state variable and $c(t)$ is the control variable.
The change in $u(t)$ over time follows the pattern $du(t)/dt = a \cdot c(t) \cdot u(t) + b$.
Considering $u(t)$ changes with time, we use this ODE: $du(t)/dt = a \cdot c(t) \cdot u(t) + b$.
The unique ODE, $du(t)/dt = a \cdot c(t) \cdot u(t) + b$ shows the variation of $u(t)$ over time affected by $c(t)$.
The ODE is in the form of $\frac{du(t)}{dt} = a \cdot c(t) \cdot u(t) + b$, where $u(t)$ is the state variable and $c(t)$ is the control variable.
The differential equation describes the change in $u(t)$ with time, expressed as $du(t)/dt = a \cdot c(t) \cdot u(t) + b$.
The ordinary differential equation governing the system is represented as $\frac{du(t)}{dt} = a \cdot c(t) \cdot u(t) + b$ where $u(t)$ and $c(t)$ are the state and control variables respectively.
Our ODE represents the time derivative of $u$ as a function of itself and a control parameter $c$, all modulated by the constants $a$ and $b$.
The dynamics of the function $u(t)$ are governed by the ordinary differential equation $\frac{du(t)}{dt} = a \cdot c(t) \cdot u(t) + b$.
The instantaneous change in $u(t)$ is dictated by the ODE via the linear combination of the product $a \cdot c(t) \cdot u(t)$ and the constant $b$.
An ordinary differential equation describing the rate of change of the state variable $u(t)$ with respect to control variable $c(t)$.
ODE describing the evolution of a state variable $u(t)$ in relation to a control variable $c(t)$.
The differential equation mentioning $u(t)$'s role in time change is $du(t)/dt = a \cdot c(t) \cdot u(t) + b$.

The ODE $\frac{du(t)}{dt} = [0.001] \cdot c(t) \cdot u(t) + [0.002]$ highlights the relationship between state variable $u(t)$ and control variable $c(t)$.
The ODE is $du(t)/dt = [0.001] \cdot c(t) \cdot u(t) + [0.002]$ with $u(t)$ and $c(t)$ as state and control variables.
How $u(t)$ changes over time is captured by the expression $\frac{du(t)}{dt} = [0.001] \cdot c(t) \cdot u(t) + [0.002]$.
The function $u(t)$ evolves according to the ODE $\frac{du(t)}{dt} = [0.001]c(t)u(t) + [0.002]$.
The state variable $u(t)$'s time behavior is governed by the ODE $du(t)/dt = [0.001] \cdot c(t) \cdot u(t) + [0.002]$.
Given parameter values as $a = [0.001]$ and $b = [0.002]$, the ODE becomes $du(t)/dt = [0.001] \cdot c(t) \cdot u(t) + [0.002]$.
Considering the parameter values $a = [0.001], b = [0.002]$, the ODE is given by $du(t)/dt = [0.001] \cdot c(t) \cdot u(t) + [0.002]$.
$du(t)/dt = a \cdot c(t) \cdot u(t) + b$, where $b = [0.002], a = [0.001]$.
The ordinary differential equation $du(t)/dt = [0.001] \cdot c(t) \cdot u(t) + [0.002]$, where $c(t)$ is the control variable and $u(t)$ the state variable.
The time behavior of the variable $u(t)$ is determined by the equation $du(t)/dt = [0.001] \cdot c(t) \cdot u(t) + [0.002]$.
The differential equation is given by $du(t)/dt = [0.001] \cdot c(t) \cdot u(t) + [0.002]$, where $u(t)$ is the state variable and $c(t)$ the control variable.
The manner in which $u(t)$ alters is captured by the ODE $du(t)/dt = [0.001] \cdot c(t) \cdot u(t) + [0.002]$.
Given the parameters $a$ and $b$ with $a = [0.001]$ and $b = [0.002]$, the ODE is then $du(t)/dt = a \cdot c(t) \cdot u(t) + b$.
The ordinary differential equation that describes our system is $du(t)/dt = [0.001] \cdot c(t) \cdot u(t) + [0.002]$.
When $a = [0.001]$ and $b = [0.002]$, the ODE has the form $du(t)/dt = [0.001] \cdot c(t) \cdot u(t) + [0.002]$.
Given $u(t)$ is the state variable and $c(t)$ the control variable, the ODE takes the form $\frac{du(t)}{dt} = [0.001] \cdot c(t) \cdot u(t) + [0.002]$.
Our ODE is given as $du(t)/dt = [0.001] \cdot c(t) \cdot u(t) + [0.002]$, with assigned values for $a$ and $b$.
With $a = [0.001]$ and $b = [0.002]$, the expression for the ODE is $du(t)/dt = [0.001] \cdot c(t) \cdot u(t) + [0.002]$.
Using parameters $a = [0.001]$ and $b = [0.002]$, the differential equation becomes $du(t)/dt = a \cdot c(t) \cdot u(t) + b$.
The differential equations is $du(t)/dt = [0.001] \cdot c(t) \cdot u(t) + [0.002]$.
The function $u(t)$ changes over time according to the rule $du(t)/dt = [0.001] \cdot c(t) \cdot u(t) + [0.002]$.
The evolution of the state variable $u(t)$ is given by the ODE $du(t)/dt = [0.001] \cdot c(t) \cdot u(t) + [0.002]$.
Given the ordinary differential equation $du(t)/dt = [0.001] \cdot c(t) \cdot u(t) + [0.002]$, the course of the state variable $u(t)$ can be determined.
The time evolution of variable $u(t)$, with parameter $c(t)$, is modeled by the ordinary differential equation $du(t)/dt = [0.001] \cdot c(t) \cdot u(t) + [0.002]$.
The ODE that describes $u(t)$'s variation with time is $du(t)/dt = [0.001] \cdot c(t) \cdot u(t) + [0.002]$.
An ordinary differential equation is defined as $\frac{du(t)}{dt} = [0.001] \cdot c(t) \cdot u(t) + [0.002]$.
We describe the ODE as $\frac{du(t)}{dt} = [0.001] \cdot c(t) \cdot u(t) + [0.002]$.
The change rate of state variable $u(t)$ is expressed as $\frac{du(t)}{dt} = [0.001] \cdot c(t) \cdot u(t) + [0.002]$.
The differential equation of the form $du(t)/dt = a \cdot c(t) \cdot u(t) + b$, with $a$ being [0.001] and $b$ being [0.002], becomes $du(t)/dt = [0.001] \cdot c(t) \cdot u(t) + [0.002]$.
In the form of an ODE, $u(t)$ is represented as $du(t)/dt = [0.001] \cdot c(t) \cdot u(t) + [0.002]$.
Given $a=[0.001]$ and $b=[0.002]$, $du(t)/dt = a \cdot c(t) \cdot u(t) + b$ is an ordinary differential equation with state variable $u(t)$ and control variable $c(t)$.
For an ODE of the form $du(t)/dt = [0.001] \cdot c(t) \cdot u(t) + [0.002]$, the state variable $u(t)$ evolves over time based on the control variable $c(t)$.
The ordinary differential equation is $\frac{du(t)}{dt} = [0.001] \cdot c(t) \cdot u(t) + [0.002]$, governing the evolution of $u(t)$.
Considering the case where $b = [0.002]$ and $a = [0.001]$, our ODE is $du(t)/dt = [0.001] \cdot c(t) \cdot u(t) + [0.002]$.
Our system is described by the ODE $du(t)/dt = [0.001] \cdot c(t) \cdot u(t) + [0.002]$.
The ODE $du(t)/dt = [0.001] \cdot c(t) \cdot u(t) + [0.002]$ depicts the modification of $u(t)$ over time with the control of variable $c(t)$.
$du(t)/dt = a \cdot c(t) \cdot u(t) + b$ is our ODE, with $a = [0.001]$ and $b = [0.002]$.
The expression of $u(t)$ in terms of differential coefficients is $du(t)/dt = [0.001] \cdot c(t) \cdot u(t) + [0.002]$.
By stating $a = [0.001]$ and $b = [0.002]$, we obtain the ODE $du(t)/dt = a \cdot c(t) \cdot u(t) + b$.
$du(t)/dt = [0.001] \cdot c(t) \cdot u(t) + [0.002]$ is the ODE defining the time evolution of the function $u(t)$ with control $c(t)$.
The ODE representing the change of $u(t)$ is $du(t)/dt = [0.001] \cdot c(t) \cdot u(t) + [0.002]$.
An ordinary differential equation typically has the form $du(t)/dt = [0.001] \cdot c(t) \cdot u(t) + [0.002]$, which models the rate of change of state variable $u(t)$.
With $a = [0.001]$ and $b = [0.002]$ the ODE expressing the transformation of $u(t)$ becomes $du(t)/dt = a \cdot c(t) \cdot u(t) + b$.
The equation $\frac{du(t)}{dt} = [0.001] \cdot c(t) \cdot u(t) + [0.002]$ explains how $u(t)$ changes with time.
The time change of $u(t)$ can be expressed by the ODE, $du(t)/dt = [0.001] \cdot c(t) \cdot u(t) + [0.002]$.
We consider the differential equation $du/dt = [0.001] \cdot c \cdot u + [0.002]$, where $u(t)$ is the state variable and $c(t)$ is the control variable.
The ODE is stated as $du(t)/dt = [0.001] \cdot c(t) \cdot u(t) + [0.002]$, featuring state variable $u(t)$ and control variable $c(t)$.
The state variable $u(t)$ evolves according to the ordinary differential equation $\frac{du(t)}{dt} = [0.001] \cdot c(t) \cdot u(t) + [0.002]$.
The equation $\frac{du(t)}{dt} = a \cdot c(t) \cdot u(t) + b$ with $a=[0.001]$ and $b=[0.002]$ models the ordinary differential equation of this system.
The differential equation $du(t)/dt = [0.001] \cdot c(t) \cdot u(t) + [0.002]$ represents a system with state variable $u(t)$ and control variable $c(t)$.
The ODE dictating the evolution of the function $u(t)$ with control $c(t)$ is $du(t)/dt = [0.001] \cdot c(t) \cdot u(t) + [0.002]$.
Function $u(t)$ changes over time as per $du(t)/dt = [0.001] \cdot c(t) \cdot u(t) + [0.002]$.
$du(t)/dt = [0.001] \cdot c(t) \cdot u(t) + [0.002]$, where the parameters $a$ and $b$ take the given values.
The status of $u(t)$ over time, manipulated by control variable $c(t)$, is represented as $du(t)/dt = [0.001] \cdot c(t) \cdot u(t) + [0.002]$.
Specified ODE: $du(t)/dt = a \cdot c(t) \cdot u(t) + b$, with $a = [0.001]$ and $b = [0.002]$.
An ODE describing the relationship between time, state variable $u(t)$, and control variable $c(t)$ is given by $du(t)/dt = [0.001] \cdot c(t) \cdot u(t) + [0.002]$.
In this ODE, we see $du(t)/dt = [0.001] \cdot c(t) \cdot u(t) + [0.002]$.
Differential equation $du(t)/dt = a \cdot c(t) \cdot u(t) + b$ where $a = [0.001]$ and $b = [0.002]$ describes the system.
For the ODE with the state variable $u(t)$ and the given parameters $a = [0.001]$ and $b = [0.002]$, we have $du(t)/dt = a \cdot c(t) \cdot u(t) + b$.
We consider the specific ODE $du(t)/dt = [0.001] \cdot c(t) \cdot u(t) + [0.002]$, where $b = [0.002]$ and $a = [0.001]$.
Here the rate of change of $u(t)$ is given by $du(t)/dt = [0.001] \cdot c(t) \cdot u(t) + [0.002]$.
In this ODE, $u(t)$ changes as per $du(t)/dt = [0.001] \cdot c(t) \cdot u(t) + [0.002]$.
The rate at which $u(t)$ varies can be described by the differential equation $du(t)/dt = [0.001] \cdot c(t) \cdot u(t) + [0.002]$.
The ODE $du(t)/dt = a \cdot c(t) \cdot u(t) + b$ becomes $du(t)/dt = [0.001] \cdot c(t) \cdot u(t) + [0.002]$, given that $a = [0.001]$ and $b = [0.002]$.
The mode of $u(t)$'s evolution over time is given by $du(t)/dt = [0.001] \cdot c(t) \cdot u(t) + [0.002]$.
The rate of change of $u(t)$ is expressed as $du(t)/dt = [0.001] \cdot c(t) \cdot u(t) + [0.002]$.
Consider the differential equation $\frac{du(t)}{dt} = [0.001] \cdot c(t) \cdot u(t) + [0.002]$ for the state variable $u(t)$ and control variable $c(t)$.
The evolution of the state variable $u(t)$ is dictated by the ODE $du(t)/dt = [0.001] \cdot c(t) \cdot u(t) + [0.002]$.
The ODE $du(t)/dt = [0.001] \cdot c(t) \cdot u(t) + [0.002]$, expresses the rate of change of state variable $u(t)$ as a function of $c(t)$.
Given the ODE $du/dt = [0.001] \cdot c \cdot u + [0.002]$ for a system with state variable $u(t)$ and control variable $c(t)$.
Our specific example of an ODE, $du(t)/dt = a \cdot c(t) \cdot u(t) + b$, is given with $a = [0.001]$ and $b = [0.002]$.
The state variable $u(t)$ obeys the differential equation $\frac{du(t)}{dt} = [0.001] \cdot c(t) \cdot u(t) + [0.002]$.
Having defined $a = [0.001]$ and $b = [0.002]$, the ODE becomes $du(t)/dt = [0.001] \cdot c(t) \cdot u(t) + [0.002]$.
The equation $du(t)/dt = [0.001] \cdot c(t) \cdot u(t) + [0.002]$ represents the change in the state variable with time.
With the parameters $a = [0.001]$ and $b = [0.002]$, the ODE is given by $du(t)/dt = a \cdot c(t) \cdot u(t) + b$.
The change in $u(t)$ is governed by the ODE $du(t)/dt = [0.001] \cdot c(t) \cdot u(t) + [0.002]$.
According to the ordinary differential equation, $u(t)$ changes with time as per $du(t)/dt = [0.001] \cdot c(t) \cdot u(t) + [0.002]$.
The function $u(t)$ follows the differential equation $du(t)/dt = a \cdot c(t) \cdot u(t) + b$, which simplifies to $du(t)/dt = [0.001] \cdot c(t) \cdot u(t) + [0.002]$.
The time-dependent equation for $u(t)$ is $\frac{du(t)}{dt} = [0.001] \cdot c(t) \cdot u(t) + [0.002]$.
Function $u(t)$ evolves over time based on $du(t)/dt = [0.001] \cdot c(t) \cdot u(t) + [0.002]$.
The ODE is defined by $du(t)/dt = a \cdot c(t) \cdot u(t) + b$ where $a = [0.001]$, $b = [0.002]$.
For the given parameters $a = [0.001]$ and $b = [0.002]$, the ODE is $\frac{du(t)}{dt} = a \cdot c(t) \cdot u(t) + b$.
The behavior of $u(t)$ over time is modeled by the ODE $du(t)/dt = [0.001] \cdot c(t) \cdot u(t) + [0.002]$.
The ODE is defined as $\frac{du(t)}{dt} = a \cdot c(t) \cdot u(t) + b$, with $a = [0.001]$ and $b = [0.002]$.
Under the ordinary differential equation $du(t)/dt = [0.001] \cdot c(t) \cdot u(t) + [0.002]$, $u(t)$ is the state variable and $c(t)$ is the control variable. 
Time-dependent $u(t)$ is denoted by $\frac{du(t)}{dt} = [0.001] \cdot c(t) \cdot u(t) + [0.002]$.
In the given ODE $du(t)/dt = [0.001] \cdot c(t) \cdot u(t) + [0.002]$, $u(t)$ is the state variable while $c(t)$ is the control variable.
The equation $du(t)/dt = a \cdot c(t) \cdot u(t) + b$ describes the state and control variables with constants $a = [0.001]$ and $b = [0.002]$.
As $u(t)$ evolves with time, its governing equation is $\frac{du(t)}{dt} = [0.001] \cdot c(t) \cdot u(t) + [0.002]$.
With $u(t)$ as the state variable, the differential equation becomes $du(t)/dt = [0.001] \cdot c(t) \cdot u(t) + [0.002]$.
For this ordinary differential equation, we use the equation $\frac{du(t)}{dt} = a \cdot c(t) \cdot u(t) + b$, with $a=[0.001]$ and $b=[0.002]$.
State variable $u(t)$ changing over time given the control variable $c(t)$ is defined by the ODE $du(t)/dt = [0.001] \cdot c(t) \cdot u(t) + [0.002]$.
The change in the state variable $u(t)$ follows the differential equation $du(t)/dt = [0.001] \cdot c(t) \cdot u(t) + [0.002]$.
For the specific values $a = [0.001], b = [0.002]$, the ODE is represented as $du(t)/dt = [0.001] \cdot c(t) \cdot u(t) + [0.002]$.
$du(t)/dt = [0.001] \cdot c(t) \cdot u(t) + [0.002]$ is the ordinary differential equation corresponding to variable $u(t)$.
Given $a = [0.001]$, $b = [0.002]$, the differential equation becomes $du(t)/dt = [0.001] \cdot c(t) \cdot u(t) + [0.002]$.
Setting $a = [0.001]$ and $b = [0.002]$, our ODE turns into $du(t)/dt = [0.001] \cdot c(t) \cdot u(t) + [0.002]$.
The ODE is expressed as $\frac{du(t)}{dt} = a \cdot c(t) \cdot u(t) + b$ where $a = [0.001]$ and $b = [0.002]$.
We have an ODE express as $du(t)/dt = a \cdot c(t) \cdot u(t) + b$, where both $a$ and $b$ are constants equal to $[0.001]$ and $[0.002]$ respectively.
The ODE is as follows: $du(t)/dt = a \cdot c(t) \cdot u(t) + b$, where $a=[0.001]$ and $b=[0.002]$.